Move ind_def examples file (which now build, thanks Peter!) to examples/ind_def so that we have one copy of these examples not two. The directory src/IndDef/examples goes away.  The clScript from the src directory doesn't go over, because the one in examples has evolved a fair bit (and now lies behind the Tutorial chapter).

examples/ind_def/opsemScript.sml
@@ -1,5 +1,5 @@
 (* =====================================================================*)
-(* FILE		: opsem.sml						*)
+(* FILE		: opsemScript.sml					*)
 (* DESCRIPTION   : Creates a theory of the syntax and operational 	*)
 (* 		  semantics of a very simple imperative programming 	*)
 (* 		  language.  Illustrates the inductive definitions 	*)
@@ -14,14 +14,17 @@
 (* =====================================================================*)
 
 (* Interactive prelude
-  app load ["stringLib", "IndDefLib", "bossLib"];
+  app load ["stringLib", "bossLib"];
 *)
 
 
 structure opsemScript =
 struct
 
-open HolKernel Parse boolLib bossLib stringLib IndDefLib IndDefRules;
+open HolKernel Parse boolLib 
+     stringLib bossLib IndDefRules; 
+
+infix ## |-> THEN THENL;  infixr 3 -->;
 
 
 (* ---------------------------------------------------------------------*)
@@ -39,7 +42,7 @@ val _ = new_theory "opsem";
 (* modelled by functions from program variables to natural numbers.	 *)
 (* --------------------------------------------------------------------- *)
 
-val state = ``:string->num``;
+val state = Type`:string->num`;
 
 (* --------------------------------------------------------------------- *)
 (* Natural number expressions and boolean expressions will just be 	 *)
@@ -48,17 +51,24 @@ val state = ``:string->num``;
 (* example on defining the semantics of commands.			 *)
 (* --------------------------------------------------------------------- *)
 
-val nexp = ``:^state -> num``
-val bexp = ``:^state -> bool``;
+val nexp = Type`:^state -> num`;
+val bexp = Type`:^state -> bool`;
+
+(*---------------------------------------------------------------------------
+     Lift type antiquotes so they can be used in term quotations. 
+ ---------------------------------------------------------------------------*)
+
+val State = ty_antiq state;
+val Bexp  = ty_antiq bexp;
 
 (* ---------------------------------------------------------------------*)
 (* We can now use the recursive types package to define the syntax of   *)
 (* commands (or "programs').  We have the following types of commands:  *)
 (*									*)
-(*    C ::=   Skip                     (does nothing)			*)
+(*    C ::=   skip                     (does nothing)			*)
 (*          | V := E                   (assignment)          		*)
 (*          | C1 ; C2                  (sequencing)           		*)
-(*          | If B then C1 else C2     (conditional)			*)
+(*          | if B then C1 else C2     (conditional)			*)
 (*          | While B do C             (repetition)			*)
 (*                                                                      *)
 (* where V ranges over program variables, E ranges over natural number	*)
@@ -70,24 +80,21 @@ val bexp = ``:^state -> bool``;
 (*						                        *)
 (*    V := E                  represented by `assign V E`		*)
 (*    C1 ; C2                 represented by `seq C1 C2`		*)
-(*    if B then C1 else C2    represented by `If B C1 C2`		*)
+(*    if B then C1 else C2    represented by `if B C1 C2`		*)
 (*    While B do C            represented by `While B C`		*)
 (*									*)
 (* ---------------------------------------------------------------------*)
 
-val _ = Hol_datatype
-          `comm
-             = Skip
-             | Assign   of string => ^nexp
-             | Seq    of  comm => comm
+val _ = Hol_datatype 
+          `comm 
+             = Skip 
+             | ::=    of string => ^nexp 
+             | ;;    of  comm => comm
              | If    of ^bexp => comm => comm
              | While of ^bexp => comm`;
 
-val _ = overload_on("<-", ``Assign``);
-val _ = overload_on(";;", ``Seq``);
-
-val _ = set_fixity "<-" (Infixr 400);
-val _ = set_fixity ";;" (Infixr 350);
+val _ = (set_fixity "::=" (Infixr 400); set_MLname "::=" "assign_def");
+val _ = (set_fixity ";;"  (Infixr 350); set_MLname ";;"  "seq_def");
 
 (* ===================================================================== *)
 (* Definition of the operational semantics.				 *)
@@ -107,25 +114,45 @@ val _ = set_fixity ";;" (Infixr 350);
 (* inductively by the set of rules shown below.  			*)
 (* ---------------------------------------------------------------------*)
 
-val State = ty_antiq state;
-val Bexp = ty_antiq bexp;
+val (rules,induction,ecases) = Hol_reln
+     `(!s. EVAL Skip s s) 
+ /\   (!s V E. EVAL (V ::= E) s (\v. if v=V then E s else s v))
+ /\   (!C1 C2 s1 s3. 
+        (?s2. EVAL C1 s1 s2 /\ EVAL C2 s2 s3) ==> EVAL (C1;;C2) s1 s3)
+ /\   (!C1 C2 s1 s2 B. EVAL C1 s1 s2 /\  B s1 ==> EVAL (If B C1 C2) s1 s2)
+ /\   (!C1 C2 s1 s2 B. EVAL C2 s1 s2 /\ ~B s1 ==> EVAL (If B C1 C2) s1 s2)
+ /\   (!C s B.                           ~B s ==> EVAL (While B C) s s)
+ /\   (!C s1 s3 B. 
+        (?s2. EVAL C s1 s2 /\ 
+              EVAL (While B C) s2 s3 /\ B s1) ==> EVAL (While B C) s1 s3)`;
 
-val (rules,induction,ecases) =
- Hol_reln
-  `(!s. EVAL Skip s s) /\
-   (!s V E. EVAL (V <- E) s (\v. if v=V then E s else s v)) /\
-   (!s1 s2 s3 C1 C2.EVAL C1 s1 s2 /\ EVAL C2 s2 s3 ==> EVAL (C1;;C2) s1 s3) /\
-   (!s1 s2 B C1 C2. EVAL C1 s1 s2 /\ B s1 ==> EVAL (If B C1 C2) s1 s2) /\
-   (!s1 s2 B C1 C2. EVAL C2 s1 s2 /\ ~B s1 ==> EVAL (If B C1 C2) s1 s2) /\
-   (!s B C. ~B s ==> EVAL (While B C) s s) /\
-   (!s1 s2 s3 B C. EVAL C s1 s2 /\ EVAL (While B C) s2 s3 /\ B s1
-                     ==> EVAL (While B C) s1 s3)`;
+val rulel = CONJUNCTS rules;
+
+(*---------------------------------------------------------------------------
+      Note that the following input is also acceptable to the 
+      definition package (existentials on the left of implications
+      have been made into universals). This is in some way
+      cleaner, but some of the following proofs depend on the 
+      specific structure of formulas and therefore fail with the
+      different representation.
+
+       (!s. EVAL Skip s s) 
+   /\  (!s V E. EVAL (V ::= E) s (\v. if v=V then E s else s v))
+   /\  (!C1 C2 s1 s2 s3. 
+                EVAL C1 s1 s2 /\ EVAL C2 s2 s3 ==> EVAL (C1;;C2) s1 s3)
+   /\  (!C1 C2 s1 s2 B. EVAL C1 s1 s2 /\  B s1 ==> EVAL (If B C1 C2) s1 s2)
+   /\  (!C1 C2 s1 s2 B. EVAL C2 s1 s2 /\ ~B s1 ==> EVAL (If B C1 C2) s1 s2)
+   /\  (!C s B.                           ~B s ==> EVAL (While B C) s s)
+   /\  (!C s1 s2 s3 B. EVAL C s1 s2 /\ 
+                EVAL (While B C) s2 s3 /\ B s1 ==> EVAL (While B C) s1 s3)
+ ---------------------------------------------------------------------------*)
+
 
 (* --------------------------------------------------------------------- *)
 (* Stronger form of rule induction.					 *)
 (* --------------------------------------------------------------------- *)
 
-val sind = derive_strong_induction(CONJUNCTS rules,induction);
+val sind = derive_strong_induction(rules,induction);
 
 (* ---------------------------------------------------------------------*)
 (* Construct the standard rule induction tactic for EVAL.  This uses	*)
@@ -137,9 +164,8 @@ val sind = derive_strong_induction(CONJUNCTS rules,induction);
 (* constructed on the fly.						*)
 (* ---------------------------------------------------------------------*)
 
-val RULE_INDUCT_TAC =
+val RULE_INDUCT_TAC = 
     RULE_INDUCT_THEN induction STRIP_ASSUME_TAC STRIP_ASSUME_TAC;
-
 
 (* =====================================================================*)
 (* Derivation of backwards case analysis theorems for each rule.        *)
@@ -151,7 +177,7 @@ val RULE_INDUCT_TAC =
 (*									*)
 (*    1: EVAL C s1 s2 							*)
 (*									*)
-(* for a specific command C (e.g. for C = `Skip`) that the              *)
+(* for a specific command C (e.g. for C = (--`Skip`--)) that the        *)
 (* corresponding instance of the premisses of the rule(s) for C must    *)
 (* also hold, since  (1) can hold only by virtue of being derivable by  *)
 (* the rule for C. This kind of reasoning occurs frequently in proofs   *)
@@ -160,13 +186,64 @@ val RULE_INDUCT_TAC =
 (* distinct, a fact automatically proved by the recursive types package.*)
 (* =====================================================================*)
 
+(* ---------------------------------------------------------------------*)
+(* The following rule is used to simplify special cases of the general  *)
+(* exhaustive case analysis theorem, which looks something like:	*)
+(*									*)
+(*      |- !C s1 s2.							*)
+(*          EVAL C s1 s2 =						*)
+(*             (C = Skip) ... \/					*)
+(*             (?V E. (C = V ::= E) ...) \/				*)
+(*             (?C1 C2 s2'. (C = C1 ; C2) ...) \/			*)
+(*             (?C1 B C2. (C = If B C1 C2) /\ B s1 ...) \/		*)
+(*             (?C2 B C1. (C = If B C1 C2) /\ ~B s1 ...) \/		*)
+(*             (?B C'. (C = While B C') /\ ~B s1 ... ) \/		*)
+(*             (?C' B s2'. (C = While B C') /\ B s1 ...)		*)
+(*  									*)
+(* If C is specialized to some particular syntactic form, for example   *)
+(* to `C1;;C2`, then most of the disjuncts in the conclusion become     *)
+(* just false because of the syntactic inequality of different commands.*)
+(* These false can be simplified away by rewriting with the theorem	*)
+(* distinct.  The disjuncts that match the command to which C is 	*)
+(* specialized can also be simplified by rewriting with const11.  This  *)
+(* changes equalities between similar commands, for example:		*)
+(*									*)
+(*    (C1 ;; C2) = (C1' ;; C2')						*)
+(*									*)
+(* to equalities between their coresponding constitutents:		*)
+(*									*)
+(*    C1 = C1'  /\  C2 = C2'						*)
+(*									*)
+(* These can then generally be used for substitution.			*)
+(* ---------------------------------------------------------------------*)
 
-val (distinct,const11) =
-  let val thm1 = TypeBase.distinct_of "comm"
-      val thm2 = TypeBase.one_one_of "comm"
-  in
+val (distinct,const11) = 
+  let val (SOME facts) = TypeBase.read {Thy="opsem", Tyop="comm"}
+      val thm1 = TypeBase.distinct_of ``:comm``
+      val thm2 = TypeBase.one_one_of ``:comm``
+  in 
     (CONJ thm1 (GSYM thm1),thm2)
   end;
+
+val SIMPLIFY = REWRITE_RULE [distinct, const11];
+
+(* --------------------------------------------------------------------- *)
+(* CASE_TAC : this is applicable to goals of the form:			 *)
+(*									 *)
+(*      TRANS C s1 s2 ==> P						 *)
+(*									 *)
+(* When applied to such a goal, the antecedant is matched to the general *)
+(* case analysis theorem and a corresponding instance of its conclusion  *)
+(* is obtained.  This is simplified using the SIMPLIFY rule described    *)
+(* above and the result is assumed in stripped form.  Given this tactic, *)
+(* the sequence of theorems given below are simple to prove.  The proofs *)
+(* are fairly uniform; with a careful analysis of the regularities, one  *)
+(* should be able to devise an automatic proof procedure for deriving    *)
+(* sets of theorems of this type.					 *)
+(* --------------------------------------------------------------------- *)
+
+val CASE_TAC = DISCH_THEN 
+               (STRIP_ASSUME_TAC o SIMPLIFY o ONCE_REWRITE_RULE[ecases]);
 
 (* --------------------------------------------------------------------- *)
 (* SKIP_THM : EVAL Skip s1 s2 is provable only by the Skip rule, which   *)
@@ -174,37 +251,38 @@ val (distinct,const11) =
 (* --------------------------------------------------------------------- *)
 
 val SKIP_THM = store_thm("SKIP_THM",
- (--`!s1 s2. EVAL Skip s1 s2 = (s1 = s2)`--),
- REPEAT (GEN_TAC ORELSE EQ_TAC) 
- THENL [ONCE_REWRITE_TAC [ecases] THEN RW_TAC std_ss [],
-        PROVE_TAC [rules]]);
+     (--`!s1 s2. EVAL Skip s1 s2 = (s1 = s2)`--),
+     REPEAT GEN_TAC THEN EQ_TAC THENL
+     [CASE_TAC THEN ASM_REWRITE_TAC [],
+      DISCH_THEN SUBST1_TAC THEN MAP_FIRST RULE_TAC rulel]);
+
 
 (* --------------------------------------------------------------------- *)
-(* ASSIGN_THM : EVAL (V <- E) s1 s2 is provable only by the assignment	 *)
+(* ASSIGN_THM : EVAL (V ::= E) s1 s2 is provable only by the assignment	 *)
 (* rule, which requires that s2 be the state s1 with V updated to E.	 *)
 (* --------------------------------------------------------------------- *)
 
-val ASSIGN_THM = store_thm 
-("ASSIGN_THM",
- --`!s1 s2 V E. EVAL (V <- E) s1 s2 
-                  =
-               ((\v. if v=V then  E s1 else s1 v) = s2)`--,
- REPEAT (GEN_TAC ORELSE EQ_TAC) 
- THENL [ONCE_REWRITE_TAC [ecases] THEN RW_TAC std_ss [], 
-        RW_TAC std_ss [] THEN RW_TAC std_ss [rules]]);
+val ASSIGN_THM = store_thm ("ASSIGN_THM",
+ (--`!s1 s2 V E. EVAL (V ::= E) s1 s2 
+                   = 
+                 ((\v. if v=V then E s1 else s1 v) = s2)`--),
+     REPEAT GEN_TAC THEN EQ_TAC THENL
+     [CASE_TAC THEN ASM_REWRITE_TAC [],
+      DISCH_THEN (SUBST1_TAC o SYM) THEN MAP_FIRST RULE_TAC rulel]);
 
 
 (* --------------------------------------------------------------------- *)
-(* SEQ_THM : EVAL (C1;C2) s1 s2 is provable only by the sequencing rule, *)
-(* which requires that some intermediate state s3 exists such that C1    *)
-(* in state s1 terminates in s3 and C3 in s3 terminates in s2.		 *)
+(* SEQ_THM : EVAL (C1;;C2) s1 s2 is provable only by the sequencing      *)
+(* rule, which requires that some intermediate state s3 exists such      *)
+(* that C1 in state s1 terminates in s3 and C3 in s3 terminates in s2.   *)
 (* --------------------------------------------------------------------- *)
 
 val SEQ_THM = store_thm("SEQ_THM",
---`!s1 s2 C1 C2.EVAL (C1;;C2) s1 s2 = (?s3. EVAL C1 s1 s3 /\ EVAL C2 s3 s2)`--,
- REPEAT (GEN_TAC ORELSE EQ_TAC)
- THENL [DISCH_THEN(MP_TAC o ONCE_REWRITE_RULE[ecases]) THEN RW_TAC std_ss [],
-        PROVE_TAC [rules]]);
+--`!s1 s2 C1 C2.EVAL (C1;;C2) s1 s2 = ?s3. EVAL C1 s1 s3 /\ EVAL C2 s3 s2`--,
+  REPEAT GEN_TAC THEN EQ_TAC THENL
+  [CASE_TAC THEN EXISTS_TAC (--`s2':^State`--) THEN ASM_REWRITE_TAC [],
+   DISCH_THEN (fn th => MAP_FIRST RULE_TAC rulel THEN MATCH_ACCEPT_TAC th)]);
+
 
 (* --------------------------------------------------------------------- *)
 (* IF_T_THM : if B(s1) is true, then EVAL (If B C2 C2) s1 s2 is provable *)
@@ -213,27 +291,27 @@ val SEQ_THM = store_thm("SEQ_THM",
 (* --------------------------------------------------------------------- *)
 
 val IF_T_THM = store_thm ("IF_T_THM",
---`!s1 s2 B C1 C2. B s1 ==> (EVAL (If B C1 C2) s1 s2 = EVAL C1 s1 s2)`--,
- REPEAT (GEN_TAC ORELSE EQ_TAC ORELSE DISCH_TAC)
- THENL [RULE_ASSUM_TAC (ONCE_REWRITE_RULE[ecases]) 
-          THEN RW_TAC std_ss []
-          THEN PROVE_TAC [],
-        PROVE_TAC [rules]]);
+(--`!s1 s2 B C1 C2. B s1 ==> (EVAL (If B C1 C2) s1 s2 = EVAL C1 s1 s2)`--),
+     REPEAT STRIP_TAC THEN EQ_TAC THENL
+     [CASE_TAC THEN EVERY_ASSUM (TRY o SUBST_ALL_TAC) THENL
+      [FIRST_ASSUM ACCEPT_TAC, RES_TAC],
+      DISCH_TAC THEN MAP_FIRST RULE_TAC rulel THEN FIRST_ASSUM ACCEPT_TAC]);
 
 
 (* --------------------------------------------------------------------- *)
-(* IF_F_THM : if B(s1) is false, then EVAL (If B C1 C2) s1 s2 is 	 *)
+(* IF_F_THM : if B(s1) is false, then EVAL (if B C1 C2) s1 s2 is 	 *)
 (* provable only by the second conditional rule, which requires that C2	 *)
 (* when evaluated in s1 terminates in s2.				 *)
 (* --------------------------------------------------------------------- *)
 
 val IF_F_THM = store_thm ("IF_F_THM",
 (--`!s1 s2 B C1 C2. ~B s1 ==> (EVAL (If B C1 C2) s1 s2 = EVAL C2 s1 s2)`--),
- REPEAT (GEN_TAC ORELSE EQ_TAC ORELSE DISCH_TAC)
- THENL [RULE_ASSUM_TAC (ONCE_REWRITE_RULE[ecases]) 
-          THEN RW_TAC std_ss []
-          THEN PROVE_TAC [],
-        PROVE_TAC [rules]]);
+   REPEAT STRIP_TAC THEN EQ_TAC THENL
+   [CASE_TAC THEN EVERY_ASSUM (TRY o SUBST_ALL_TAC) THENL
+    [RES_TAC, FIRST_ASSUM ACCEPT_TAC],
+     DISCH_TAC THEN MAP_FIRST RULE_TAC (rev rulel) THEN
+     FIRST_ASSUM ACCEPT_TAC]);
+
 
 (* ---------------------------------------------------------------------*)
 (* WHILE_T_THM : if B(s1) is true, then EVAL (While B C) s1 s2 is 	*)
@@ -243,15 +321,17 @@ val IF_F_THM = store_thm ("IF_F_THM",
 (* ---------------------------------------------------------------------*)
 
 val WHILE_T_THM = store_thm ("WHILE_T_THM",
---`!s1 s2 B C. 
-     B s1 ==> (EVAL (While B C) s1 s2 
-                 =
-              ?s3. EVAL C s1 s3 /\ EVAL (While B C) s3 s2)`--,
- REPEAT (STRIP_TAC ORELSE EQ_TAC)
- THENL [RULE_ASSUM_TAC (ONCE_REWRITE_RULE[ecases]) 
-          THEN RW_TAC std_ss [],
-        ALL_TAC]
- THEN PROVE_TAC [rules]);
+     (--`!s1 s2 B C.
+      B s1 ==> (EVAL (While B C) s1 s2 =
+                (?s3. EVAL C s1 s3 /\ EVAL (While B C) s3 s2))`--),
+   REPEAT STRIP_TAC THEN EQ_TAC THENL
+   [CASE_TAC THEN EVERY_ASSUM (TRY o SUBST_ALL_TAC) THENL
+    [RES_TAC,
+     EXISTS_TAC (--`s2':^State`--) THEN CONJ_TAC THEN FIRST_ASSUM ACCEPT_TAC],
+    STRIP_TAC THEN MAP_FIRST RULE_TAC (rev rulel) THEN
+    EXISTS_TAC (--`s3:^State`--) THEN
+    REPEAT CONJ_TAC THEN FIRST_ASSUM ACCEPT_TAC]);
+
 
 (* ---------------------------------------------------------------------*)
 (* WHILE_F_THM : if B(s1) is false, then EVAL (While B C) s1 s2 is	*)
@@ -260,12 +340,14 @@ val WHILE_T_THM = store_thm ("WHILE_T_THM",
 (* ---------------------------------------------------------------------*)
 
 val WHILE_F_THM = store_thm ("WHILE_F_THM",
---`!s1 s2 B C. ~B s1 ==> (EVAL (While B C) s1 s2 = (s1 = s2))`--,
- REPEAT (STRIP_TAC ORELSE EQ_TAC)
- THENL [RULE_ASSUM_TAC (ONCE_REWRITE_RULE[ecases]) 
-          THEN RW_TAC std_ss [],
-        ALL_TAC]
- THEN PROVE_TAC [rules]);
+     (--`!s1 s2 B C. ~B s1 ==> (EVAL (While B C) s1 s2 = (s1 = s2))`--),
+     REPEAT STRIP_TAC THEN EQ_TAC THENL
+     [CASE_TAC THENL
+      [CONV_TAC SYM_CONV THEN FIRST_ASSUM ACCEPT_TAC,
+       EVERY_ASSUM (TRY o SUBST_ALL_TAC) THEN RES_TAC],
+      DISCH_THEN (SUBST1_TAC o SYM) THEN MAP_FIRST RULE_TAC rulel THEN
+      FIRST_ASSUM ACCEPT_TAC]);
+
 
 (* ===================================================================== *)
 (* THEOREM: the operational semantics is deterministic.			 *)
@@ -278,25 +360,57 @@ val WHILE_F_THM = store_thm ("WHILE_F_THM",
 (* ===================================================================== *)
 
 val DETERMINISTIC = store_thm ("DETERMINISTIC",
---`!C st1 st2. EVAL C st1 st2 ==> !st3. EVAL C st1 st3 ==> (st2 = st3)`--,
-  RULE_INDUCT_TAC THEN REPEAT GEN_TAC 
-  THEN RW_TAC std_ss 
-     [SKIP_THM,ASSIGN_THM,SEQ_THM,IF_T_THM, IF_F_THM, WHILE_F_THM,WHILE_T_THM]
-  THEN PROVE_TAC []);
+(--`!C st1 st2. EVAL C st1 st2 ==> !st3. EVAL C st1 st3 ==> (st2 = st3)`--),
+     RULE_INDUCT_TAC THEN REPEAT GEN_TAC THENL
+     [REWRITE_TAC [SKIP_THM],
+      REWRITE_TAC [ASSIGN_THM],
+      PURE_ONCE_REWRITE_TAC [SEQ_THM] THEN STRIP_TAC THEN
+      FIRST_ASSUM MATCH_MP_TAC THEN RES_TAC THEN ASM_REWRITE_TAC [],
+      IMP_RES_TAC IF_T_THM THEN ASM_REWRITE_TAC [],
+      IMP_RES_TAC IF_F_THM THEN ASM_REWRITE_TAC [],
+      IMP_RES_TAC WHILE_F_THM THEN ASM_REWRITE_TAC [],
+      IMP_RES_THEN (fn th =>  PURE_ONCE_REWRITE_TAC [th]) WHILE_T_THM THEN
+      STRIP_TAC THEN FIRST_ASSUM MATCH_MP_TAC THEN
+      RES_TAC THEN ASM_REWRITE_TAC []]);
 
 
 (* ===================================================================== *)
 (* Definition of partial correctness and derivation of proof rules.	 *)
 (* ===================================================================== *)
 
-val SPEC_DEF = 
- new_definition 
-   ("SPEC_DEF",
-    --`SPEC P C Q = !s1 s2. (P s1 /\ EVAL C s1 s2) ==> Q s2`--);
+val SPEC_DEF = new_definition ("SPEC_DEF",
+     (--`SPEC P C Q = !s1 s2. (P s1 /\ EVAL C s1 s2) ==> Q s2`--));
 
 (* --------------------------------------------------------------------- *)
 (* Proof of the While rule in Hoare logic.				 *)
 (* --------------------------------------------------------------------- *)
+
+(* --------------------------------------------------------------------- *)
+(* In the following proofs, theorems of the form:			 *)
+(*									 *)
+(*     |- !y1...yn. (C x1 ... xn = C y1 ... yn) ==> tm[y1,...,yn]	 *)
+(*									 *)
+(* frequently arise, where C is one of the constructors of the data type *)
+(* of commands.  The following theorem-tactic simplifies such theorems   *)
+(* by specializing yi to xi and then removing the resulting trivially    *)
+(* true antecedent.  The result is:					 *)
+(*									 *)
+(*     |- tm[x1,...,xn/y1,...,yn]					 *)
+(*									 *)
+(* which is passed to the theorem continuation function. The tactic just *)
+(* discards theorems not of the form shown above.   For the While proof  *)
+(* given below, this has the effect of thinning out useless induction	 *)
+(* hypotheses of the form:						 *)
+(*									 *)
+(*     |- !B' C'. (C = While B' C') ==> tm[B',C']			 *)
+(* 									 *)
+(* These are just discarded.						 *)
+(* --------------------------------------------------------------------- *)
+
+fun REFL_MP_THEN ttac th =
+   let val tm = lhs(fst(dest_imp(snd(strip_forall(concl th)))))
+   in ttac (MATCH_MP th (REFL tm))
+   end handle HOL_ERR _ => ALL_TAC;
 
 (* --------------------------------------------------------------------- *)
 (* The following lemma states that the condition B in While B C must be  *)
@@ -321,13 +435,17 @@ val SPEC_DEF =
 (* Showing that the above set is closed under the two While rules is     *)
 (* likewise trivial.  For the While axiom, we get ~(B s2) immediately 	 *)
 (* from the side condition. For the other While rule, the statement to	 *)
-(* prove is just one of the induction hypotheses.                        *)
+(* prove is just one of the induction hypotheses; since RULE_INDUCT_TAC  *)
+(* uses STRIP_ASSUME_TAC on this hypothesis, this subgoal is solved	 *)
+(* immediately.								 *)
 (* --------------------------------------------------------------------- *)
 
 
 val WHILE_LEMMA1 = TAC_PROOF(([],
---`!C s1 s2. EVAL C s1 s2 ==> !B' C'. (C = While B' C') ==> ~(B' s2)`--),
-  RULE_INDUCT_TAC THEN REWRITE_TAC [distinct, const11] THEN PROVE_TAC []);
+ (--`!C s1 s2. EVAL C s1 s2 ==> !B' C'. (C = While B' C') ==> ~(B' s2)`--)),
+     RULE_INDUCT_TAC THEN REWRITE_TAC [distinct, const11] THEN
+     REPEAT GEN_TAC THEN DISCH_THEN (STRIP_THM_THEN SUBST_ALL_TAC) THEN
+     FIRST_ASSUM ACCEPT_TAC);
 
 (* ---------------------------------------------------------------------*)
 (* The second lemma deals with the invariant part of the Hoare proof 	*)
@@ -353,23 +471,32 @@ val WHILE_LEMMA1 = TAC_PROOF(([],
 (* desired conclusion in the step case of the While rule.  To see why, 	*)
 (* try replacing strong by weak induction in the tactic proof below.	*)
 (*									*)
+(* Note that REFL_MP_THEN is used to simplify the induction hypotheses  *)
+(* before adding them to the assumption list.  This avoids having the 	*)
+(* assumptions in an awkward form (try using ASSUME_TAC instead). Note	*)
+(* also that in the case of the While axiom, the states s1 and s2 are	*)
+(* identical, so the corresponding subgoal is trivial and is solved by	*)
+(* the rewriting step.							*)
 (* ---------------------------------------------------------------------*)
 
 val WHILE_LEMMA2 =
     TAC_PROOF(([],
-  --`!C s1 s2.
+  --`!C s1 s2. 
      EVAL C s1 s2 ==>
      !B' C'. (C = While B' C') ==>
              (!s1 s2. P s1 /\ B' s1 /\ EVAL C' s1 s2 ==> P s2) ==>
              (P s1 ==> P s2)`--),
- HO_MATCH_MP_TAC sind THEN RW_TAC std_ss [] THEN PROVE_TAC []);
+     RULE_INDUCT_THEN sind (REFL_MP_THEN ASSUME_TAC) ASSUME_TAC THEN 
+     REWRITE_TAC [distinct, const11] THEN REPEAT GEN_TAC THEN
+     DISCH_THEN (STRIP_THM_THEN SUBST_ALL_TAC) THEN
+     REPEAT STRIP_TAC THEN RES_TAC);
 
 (* ---------------------------------------------------------------------*)
 (* The proof rule for While commands in Hoare logic is:			*)
 (*									*)
 (*         |- {P /\ B} C {P}						*)
-(*      -------------------------------					*)
-(*         |- {P} While B C {P /\ ~B}					*)
+(*      ----------------------						*)
+(*        |- {P} C {P /\ ~B}						*)
 (* 									*)
 (* Given the two lemmas proved above, it is trivial to prove this rule. *)
 (* The antecedent of the rule is just the assumption of invariance of P *)
@@ -378,12 +505,14 @@ val WHILE_LEMMA2 =
 (* ---------------------------------------------------------------------*)
 
 val WHILE = store_thm ("WHILE",
---`!P C. SPEC (\s. P s /\ B s) C P 
-         ==>
-         SPEC P (While B C) (\s. P s /\ ~B s)`--,
- RW_TAC std_ss [SPEC_DEF] 
- THENL [PROVE_TAC [WHILE_LEMMA2],
-        PROVE_TAC [WHILE_LEMMA1]]);
+     (--`!P C. SPEC (\s. P s /\ B s) C P ==>
+            SPEC P (While B C) (\s. P s /\ ~B s)`--),
+     PURE_ONCE_REWRITE_TAC [SPEC_DEF] THEN
+     CONV_TAC (ONCE_DEPTH_CONV BETA_CONV) THEN
+     PURE_ONCE_REWRITE_TAC [SYM(SPEC_ALL CONJ_ASSOC)] THEN
+     REPEAT STRIP_TAC THENL
+     [IMP_RES_THEN (REFL_MP_THEN IMP_RES_TAC) WHILE_LEMMA2,
+      IMP_RES_THEN (REFL_MP_THEN IMP_RES_TAC) WHILE_LEMMA1]);
 
 (* ---------------------------------------------------------------------*)
 (* End of example.							*)
