examples/ind_def/algebraScript.sml
@@ -1,5 +1,5 @@
 (* ===================================================================== *)
-(* File		: algebra.ml						 *)
+(* File		: algebraScript.sml                                      *)
 (* DESCRIPTION  : Maximal trace semantics and transition semantics of a  *)
 (*		  small process algebra.              			 *)
 (*									 *)
@@ -8,7 +8,7 @@
 (* ===================================================================== *)
 
 (*
-  app load ["IndDefLib", "stringLib", "bossLib"];
+  app load ["stringLib", "listTheory", "bossLib"];
 *)
 
 structure algebraScript =
@@ -19,13 +19,12 @@ struct
 (* other libraries.                                                      *)
 (* --------------------------------------------------------------------- *)
 
-open HolKernel Parse boolLib bossLib
-     IndDefLib IndDefRules listTheory;
-
 local open stringTheory in end;
 
-infixr 3 -->;
-infix ## |-> THEN THENL THENC ORELSE ORELSEC THEN_TCL ORELSE_TCL;
+open HolKernel Parse boolLib bossLib
+     IndDefRules listTheory;
+
+infix ## |-> THEN THENL ORELSE;  infixr 3 -->;
 
 
 val _ = new_theory "algebra";
@@ -53,26 +52,32 @@ val _ = new_theory "algebra";
 (* abbreviation for :string.						 *)
 (* --------------------------------------------------------------------- *)
 
-val  label = Type`:string`;
+val label = Type`:string`;
 
-val _ = Hol_datatype `agent
-                        = Nil
-                        | Pre of  ^label => agent
-                        | Sum of   agent => agent
-                        | Prod of  agent => agent`;
+val _ = Hol_datatype `agent 
+                         = Nil 
+                         | Pre of  ^label => agent
+                         | Sum of   agent => agent
+                         | Prod of  agent => agent`;
 
+
+(* ===================================================================== *)
+(* Standard syntactic theory, derived by the recursive types package.	 *)
+(* ===================================================================== *)
+
+val SOME agentfacts = TypeBase.read {Thy="algebra", Tyop="agent"};
 
 (* --------------------------------------------------------------------- *)
 (* structural induction theorem for agent.                               *)
 (* --------------------------------------------------------------------- *)
 
-val induct = TypeBase.induction_of "agent";
+val induct = TypeBase.induction_of ``:agent``;
 
 (* --------------------------------------------------------------------- *)
 (* cases theorem for agent.                                              *)
 (* --------------------------------------------------------------------- *)
 
-val cases = TypeBase.nchotomy_of "agent";
+val cases = TypeBase.nchotomy_of ``:agent``;
 
 (* --------------------------------------------------------------------- *)
 (* The constructors of the type :agent yield syntactically distinct      *)
@@ -81,9 +86,10 @@ val cases = TypeBase.nchotomy_of "agent";
 (* --------------------------------------------------------------------- *)
 
 val distinct =
-   let val ths = CONJUNCTS (TypeBase.distinct_of "agent")
+   let val distinct = TypeBase.distinct_of ``:agent``
+       val ths = CONJUNCTS distinct
        val rths = map (GEN_ALL o NOT_EQ_SYM o SPEC_ALL) ths
-   in
+   in 
      LIST_CONJ (ths @ rths)
    end;
 
@@ -91,15 +97,21 @@ val distinct =
 (* The constructors Pre, Sum and Prod are one-to-one.                    *)
 (* --------------------------------------------------------------------- *)
 
-val agent11 = CONJUNCTS (TypeBase.one_one_of "agent");
+val agent11 =
+   let val one2 = TypeBase.one_one_of ``:agent``
+   in CONJUNCTS one2
+   end;
 
 (* ===================================================================== *)
 (* Definition of a maximal trace semantics for the process algebra.	 *)
 (* ===================================================================== *)
 
 (* --------------------------------------------------------------------- *)
-(* Traces are just finite sequences of labels, represented by lists      *)
+(* Type abbreviation for traces.   These are just finite sequences of 	 *)
+(* labels, represented here by lists.					 *)
 (* --------------------------------------------------------------------- *)
+
+val trace = ty_antiq(Type`:^label list`);
 
 (* --------------------------------------------------------------------- *)
 (* Inductive definition of a trace relation MTRACE.  This is defined so	 *)
@@ -107,27 +119,21 @@ val agent11 = CONJUNCTS (TypeBase.one_one_of "agent");
 (* definition is done inductively by the rules given below.	     	 *)
 (* --------------------------------------------------------------------- *)
 
-val (trules,tind,tcases) = 
-  IndDefLib.Hol_reln
-   `(MTRACE Nil []) /\
-    (!P A a. MTRACE P A ==> MTRACE (Pre a P) (a::A)) /\
-    (!P Q A. MTRACE P A ==> MTRACE (Sum P Q) A) /\
-    (!P Q A. MTRACE Q A ==> MTRACE (Sum P Q) A) /\
-    (!P Q A. MTRACE P A /\
-             MTRACE Q A ==> MTRACE (Prod P Q) A)`;
+val (trules, tind, tcases) = Hol_reln
+     `MTRACE Nil [] 
+ /\   (!P A a. MTRACE P A ==> MTRACE (Pre a P) (a::A))
+ /\   (!P Q A. MTRACE P A ==> MTRACE (Sum P Q) A)
+ /\   (!P Q A. MTRACE Q A ==> MTRACE (Sum P Q) A)
+ /\   (!P Q A. MTRACE P A /\ MTRACE Q A ==> MTRACE (Prod P Q) A)`;
+
+
+val trulel = CONJUNCTS trules;
 
 (* --------------------------------------------------------------------- *)
 (* Stronger form of rule induction.					 *)
 (* --------------------------------------------------------------------- *)
 
-val tsind = IndDefRules.derive_strong_induction (CONJUNCTS trules,tind);
-
-(* --------------------------------------------------------------------- *)
-(* Definition of a terminal process: one with [] as a maximal trace.	 *)
-(* --------------------------------------------------------------------- *)
-
-val TERMINAL_DEF =
-    new_definition ("TERMINAL_DEF", Term`TERMINAL P = MTRACE P []`);
+val tsind = derive_strong_induction (trules,tind);
 
 (* --------------------------------------------------------------------- *)
 (* Standard rule induction tactic for MTRACE. This uses the weaker form  *)
@@ -138,29 +144,119 @@ val TERMINAL_DEF =
 val MTRACE_INDUCT_TAC =
     RULE_INDUCT_THEN tind STRIP_ASSUME_TAC STRIP_ASSUME_TAC;
 
+(* --------------------------------------------------------------------- *)
+(* Tactics for each of the rules defining MTRACE.			 *)
+(* --------------------------------------------------------------------- *)
+
+val [Nil_TAC,Pre_TAC,SumL_TAC,SumR_TAC,Prod_TAC] = map RULE_TAC trulel;
+
+(* --------------------------------------------------------------------- *)
+(* Given the tactics defined above for each rule, we now define a tactic *)
+(* that searches for a proof that a process has some particular maximal  *)
+(* trace, given some assumptions about maximal traces.  Note that there	 *)
+(* are two Sum rules, so our tactic may have to do some backtracking in  *)
+(* the proof.  In addition to seaching using the MTRACE rules, the 	 *)
+(* looks for solutions among the assumptions as well as back-chaining 	 *)
+(* with any implications among the assumptions. The tactics fails unless *)
+(* it completely solves the goal.					 *)
+(* --------------------------------------------------------------------- *)
+
+fun MTRACE_TAC g =
+   (REPEAT STRIP_TAC THEN
+    FIRST [Nil_TAC,
+           FIRST_ASSUM MATCH_ACCEPT_TAC,
+           Pre_TAC THEN MTRACE_TAC,
+           SumL_TAC THEN MTRACE_TAC,
+           SumR_TAC THEN MTRACE_TAC,
+           Prod_TAC  THEN MTRACE_TAC,
+   	   FIRST_ASSUM MATCH_MP_TAC THEN MTRACE_TAC]) g ;
+
+
+(* --------------------------------------------------------------------- *)
+(* The following is a little rule for getting simplified instances of	 *)
+(* the tcases theorem.  All it does is to specialize tcases to the 	 *)
+(* supplied process, rewrite using the distinctness and injectivity of	 *)
+(* constructors, and eliminate redundant equations using REDUCE. Examples*)
+(* of using MTCASE are:							 *)
+(*									 *)
+(*   #MTCASE (--`Prod P Q`--);						 *)
+(*   |- !P Q A. MTRACE(Prod P Q)A = MTRACE P A /\ MTRACE Q A		 *)
+(*									 *)
+(*   #MTCASE (--`Sum P Q`--);						 *)
+(*   |- !P Q A. MTRACE(Sum P Q)A = MTRACE P A \/ MTRACE Q A		 *)
+(*									 *)
+(* --------------------------------------------------------------------- *)
+
+val MTCASE =
+   let val SIMPLIFY = REWRITE_RULE (distinct :: agent11)
+   in fn tm => let val th1 = SIMPLIFY (SPEC tm tcases) 
+               in GEN_ALL (CONV_RULE (ONCE_DEPTH_CONV REDUCE) th1)
+               end
+   end;
+
+(* --------------------------------------------------------------------- *)
+(* Definition of a terminal process: one with [] as a maximal trace.	 *)
+(* --------------------------------------------------------------------- *)
+
+val TERMINAL_DEF =
+  Q.new_definition ("TERMINAL_DEF", `TERMINAL P = MTRACE P []`);
+
 (* ===================================================================== *)
 (* Inductive definition of a labelled transition system.                 *)
 (* ===================================================================== *)
 
 (* --------------------------------------------------------------------- *)
 (* We now define a labelled transition relation TRANS P l Q to mean	 *)
-(* that process P can participate in action l and thereby evolve into	 *)
-(* process Q.  The definition is done inductively, as usual.             *)
+(* there that process P can participate in action l and thereby evolve	 *)
+(* into process Q.  The definition is done inductively, as usual.        *)
 (* --------------------------------------------------------------------- *)
 
-val (lrules,lind,lcases) =
-  Hol_reln
-     `(!a Q. TRANS (Pre a Q) a Q) /\
-      (!a P P' Q. TRANS P a P' ==> TRANS (Sum P Q) a P') /\
-      (!a P Q Q'. TRANS Q a Q' ==> TRANS (Sum P Q) a Q') /\
-      (!a P P' Q Q'. TRANS P a P' /\ 
-                     TRANS Q a Q' ==> TRANS (Prod P Q) a (Prod P' Q'))`;
+val (lrules, lind, lcases) = Hol_reln
+    `(!Q a. TRANS (Pre a Q) a Q)
+ /\  (!P P' Q a. TRANS P a P' ==> TRANS (Sum P Q) a P')
+ /\  (!P Q Q' a. TRANS Q a Q' ==> TRANS (Sum P Q) a Q')
+ /\  (!P P' Q Q' a. TRANS P a P' /\ TRANS Q a Q' 
+                ==> TRANS (Prod P Q) a (Prod P' Q'))`;
+
+val lrulel = CONJUNCTS lrules;
 
 (* --------------------------------------------------------------------- *)
 (* Strong form of rule induction for TRANS.	      			 *)
 (* --------------------------------------------------------------------- *)
 
-val lsind = derive_strong_induction (CONJUNCTS lrules,lind);
+val lsind = derive_strong_induction (lrules,lind);
+
+(* --------------------------------------------------------------------- *)
+(* Standard rule induction tactic for TRANS. This again just uses the	 *)
+(* weaker form of rule induction theorem.  Both premisses and side 	 *)
+(* conditions are assumed (in stripped form).  				 *)
+(* --------------------------------------------------------------------- *)
+
+val TRANS_INDUCT_TAC =
+    RULE_INDUCT_THEN lind STRIP_ASSUME_TAC STRIP_ASSUME_TAC;
+
+(* --------------------------------------------------------------------- *)
+(* Tactics for the TRANS rules.						 *)
+(* --------------------------------------------------------------------- *)
+
+val [TPre_TAC,TSumL_TAC,TSumR_TAC,TProd_TAC] = map RULE_TAC lrulel;
+
+(* --------------------------------------------------------------------- *)
+(* Given the tactics defined above for each rule, we construct a tactic  *)
+(* that searches for a proof of TRANS P a Q, with becktracking in the 	 *)
+(* Sum case.  The tactic also looks for the solution on the assumption	 *)
+(* list of the goal, with backchaining through implications. 		 *)
+(* --------------------------------------------------------------------- *)
+
+fun TRANS_TAC g =
+   (REPEAT STRIP_TAC THEN
+    FIRST [FIRST_ASSUM MATCH_ACCEPT_TAC,
+           TPre_TAC,
+           TSumL_TAC THEN TRANS_TAC,
+           TSumR_TAC THEN TRANS_TAC,
+           TProd_TAC  THEN TRANS_TAC,
+   	   FIRST_ASSUM MATCH_MP_TAC THEN TRANS_TAC]) g;
+
 
 (* ===================================================================== *)
 (* Inductive definition of a trace transition system                	 *)
@@ -172,22 +268,32 @@ val lsind = derive_strong_induction (CONJUNCTS lrules,lind);
 (* TRANS, but with the label being a list of the labels from TRANS.	 *)
 (* --------------------------------------------------------------------- *)
 
-val (Lrules,Lind,Lcases) =
- Hol_reln
-   `(!P. TRANSIT P [] P) /\
-    (!a P P' B. (?Q. TRANS P a Q /\ TRANSIT Q B P') ==> TRANSIT P (a::B) P')`;
+val (Lrules, Lind, Lcases) = Hol_reln
+    `(!P. TRANSIT P [] P) 
+ /\  (!P P' B a. 
+         (?Q. TRANS P a Q /\ TRANSIT Q B P') ==> TRANSIT P (a::B) P')`;
+
+val Lrulel = CONJUNCTS Lrules;
 
 (* --------------------------------------------------------------------- *)
 (* Strong form of rule induction for labelled (trace) transitions.       *)
 (* --------------------------------------------------------------------- *)
 
-val Lsind = derive_strong_induction (CONJUNCTS Lrules,Lind);
+val Lsind = derive_strong_induction (Lrules,Lind);
 
 (* --------------------------------------------------------------------- *)
 (* Rule induction tactic for TRANSIT.					 *)
 (* --------------------------------------------------------------------- *)
 
 val TRANSIT_INDUCT_TAC = RULE_INDUCT_THEN Lind ASSUME_TAC ASSUME_TAC;
+
+(* --------------------------------------------------------------------- *)
+(* A tactic for each TRANSIT rule. If matching conclusions to goals,     *)
+(* the two rules are mutually exclusive---so only the following single	 *)
+(* tactic is needed.							 *)
+(* --------------------------------------------------------------------- *)
+
+val TRANSIT_TAC = MAP_FIRST RULE_TAC Lrulel;
 
 (* ===================================================================== *)
 (* Theorem 1: Maximal trace semantics "agrees' with transition semantics *)
@@ -196,7 +302,7 @@ val TRANSIT_INDUCT_TAC = RULE_INDUCT_THEN Lind ASSUME_TAC ASSUME_TAC;
 (* --------------------------------------------------------------------- *)
 (* Lemma 1 is to prove the following theorem:				 *)
 (*									 *)
-(*    |- !P a Q. TRANS P a Q ==> !A. MTRACE Q A ==> MTRACE P (CONS a A)  *)
+(*    |- !P a Q. TRANS P a Q ==> !A. MTRACE Q A ==> MTRACE P (a::A)      *)
 (*									 *)
 (* The proof is a straightforward rule induction on TRANS, followed by	 *)
 (* a case analysis on MTRACE Q A when Q is a product (Prod), and then	 *)
@@ -204,15 +310,12 @@ val TRANSIT_INDUCT_TAC = RULE_INDUCT_THEN Lind ASSUME_TAC ASSUME_TAC;
 (* the tactic MTRACE_TAC.						 *)
 (* --------------------------------------------------------------------- *)
 
-val Lemma1 = prove
-(--`!P a Q. TRANS P a Q ==> !A. MTRACE Q A ==> MTRACE P (a::A)`--,
- HO_MATCH_MP_TAC lind 
- THEN REPEAT CONJ_TAC
- THENL [ALL_TAC,ALL_TAC,ALL_TAC,
-        REPEAT GEN_TAC THEN STRIP_TAC THEN GEN_TAC 
-          THEN DISCH_THEN (MP_TAC o ONCE_REWRITE_RULE [tcases]) 
-          THEN RW_TAC std_ss []]
- THEN PROVE_TAC [trules]);
+val Lemma1 = Q.prove
+(`!P a Q. TRANS P a Q ==> !A. MTRACE Q A ==> MTRACE P (a::A)`,  
+ TRANS_INDUCT_TAC THEN REPEAT GEN_TAC THEN
+ let val PCASES = PURE_ONCE_REWRITE_RULE [MTCASE (--`Prod P Q`--)] 
+ in DISCH_THEN (STRIP_ASSUME_TAC o PCASES) THEN MTRACE_TAC
+ end);
 
 (* --------------------------------------------------------------------- *)
 (* Theorem 1:  |- !P A Q. TRANSIT P A Q ==> TERMINAL Q ==> MTRACE P A    *)
@@ -224,9 +327,13 @@ val Lemma1 = prove
 (* through a maximal trace of P.					 *)
 (* --------------------------------------------------------------------- *)
 
-val Theorem1 = store_thm ("Theorem1",
---`!P A Q. TRANSIT P A Q ==> TERMINAL Q ==> MTRACE P A`--,
-  TRANSIT_INDUCT_TAC THEN PROVE_TAC [Lemma1,TERMINAL_DEF]);
+val Theorem1 =
+    store_thm
+    ("Theorem1",
+     (--`!P A Q. TRANSIT P A Q ==> TERMINAL Q ==> MTRACE P A`--),
+     PURE_ONCE_REWRITE_TAC [TERMINAL_DEF] THEN 
+     TRANSIT_INDUCT_TAC THEN REPEAT STRIP_TAC THEN
+     RES_TAC THEN IMP_RES_TAC Lemma1);
 
 (* --------------------------------------------------------------------- *)
 (* Corollary 1: !P A Q. TRANSIT P A Nil ==> MTRACE P A                   *)
@@ -234,13 +341,51 @@ val Theorem1 = store_thm ("Theorem1",
 (* Note that the converse does not hold.				 *)
 (* --------------------------------------------------------------------- *)
 
-val Corollary1 = store_thm ("Corollary1",
-  --`!P A. TRANSIT P A Nil ==> MTRACE P A`--,
-  PROVE_TAC [Theorem1,TERMINAL_DEF,trules]);
+val Corollary1 = 
+    store_thm
+    ("Corollary1",
+     (--`!P A. TRANSIT P A Nil ==> MTRACE P A`--),
+     REPEAT STRIP_TAC THEN
+     IMP_RES_THEN MATCH_MP_TAC Theorem1 THEN
+     PURE_ONCE_REWRITE_TAC [TERMINAL_DEF] THEN
+     MTRACE_TAC);
 
 (* ===================================================================== *)
 (* Theorem 2: Transition semantics "agrees" with maximal trace semantics *)
 (* ===================================================================== *)
+
+(* --------------------------------------------------------------------- *)
+(* The following tactic is for solving existentially-quantified goals,	 *)
+(* the bodies of which are conjunctions of assertions of membership in	 *)
+(* one or more of the inductively-defined relations we're working with.  *)
+(* All it does is to reduce the goal with the supplied witness, and then *)
+(* apply the tactic for the relevant relation.				 *)
+(* --------------------------------------------------------------------- *)
+
+fun EXISTS_SEARCH_TAC tm =
+     EXISTS_TAC tm THEN REPEAT STRIP_TAC THEN
+       TRY(FIRST [TRANS_TAC, MTRACE_TAC, TRANSIT_TAC]);
+
+(* --------------------------------------------------------------------- *)
+(* A little tactic for case analysis on the trace-transition system. 	 *)
+(* When supplied with a term (--`TRANSIT P A Q`--), which should be one  *)
+(* of the assumptions of the current goal, the tactic gets the           *)
+(* corresponding instance of the TRANSIT case analysis theorem,          *)
+(* simplifies out any false case, and enriches the goal with the         *)
+(* remaining facts, either by assuming them or, in the case of equations,*)
+(* by substitution.		                                         *)
+(* --------------------------------------------------------------------- *)
+
+val TRANSIT_CASES_TAC = 
+  let fun SUBST_ASSUME th = SUBST_ALL_TAC th ORELSE STRIP_ASSUME_TAC th
+      val TTAC = REPEAT_TCL STRIP_THM_THEN SUBST_ASSUME
+  in fn tm =>
+      let val th1 = UNDISCH(fst(EQ_IMP_RULE(REWR_CONV Lcases tm)))
+          val th2 = REWRITE_RULE [NOT_CONS_NIL,NOT_NIL_CONS,CONS_11] th1 
+      in 
+        REPEAT_TCL STRIP_THM_THEN SUBST_ASSUME th2
+      end
+  end;
 
 (* --------------------------------------------------------------------- *)
 (* Lemma 2 shows that the trace of a product is just the trace of its	 *)
@@ -249,12 +394,13 @@ val Corollary1 = store_thm ("Corollary1",
 (* case analysis theorem for TRANSIT.					 *)
 (* --------------------------------------------------------------------- *)
 
-val Lemma2 = prove
-(--`!A P Q P' Q'.
-    TRANSIT P A Q /\ TRANSIT P' A Q' ==> TRANSIT (Prod P P') A (Prod Q Q')`--,
- Induct THEN PURE_ONCE_REWRITE_TAC [Lcases] 
-        THEN RW_TAC std_ss [] 
-        THEN PROVE_TAC [Lrules,lrules]);
+val Lemma2 = Q.prove
+(`!A P Q P' Q'.
+    TRANSIT P A Q /\ TRANSIT P' A Q' ==> TRANSIT (Prod P P') A (Prod Q Q')`,
+ Induct
+   THEN PURE_ONCE_REWRITE_TAC [Lcases] 
+   THEN RW_TAC std_ss []
+   THEN EXISTS_SEARCH_TAC (--`Prod Q'' Q'''`--));
 
 (* --------------------------------------------------------------------- *)
 (* Theorem 2:  |- !P A. MTRACE P A ==> ?Q. TRANSIT P A Q /\ TERMINAL Q	 *)
@@ -269,15 +415,19 @@ val Lemma2 = prove
 (* witnesses required for the two TRANSIT rules.			 *)
 (* --------------------------------------------------------------------- *)
 
-val Theorem2 = store_thm ("Theorem2",
-(--`!P A. MTRACE P A ==> ?Q. TRANSIT P A Q /\ TERMINAL Q`--),
-  PURE_ONCE_REWRITE_TAC [TERMINAL_DEF] 
-    THEN MTRACE_INDUCT_TAC
-    THENL [ALL_TAC, ALL_TAC, 
-           RULE_ASSUM_TAC(ONCE_REWRITE_RULE [Lcases]) THEN RW_TAC std_ss [],
-           RULE_ASSUM_TAC(ONCE_REWRITE_RULE [Lcases]) THEN RW_TAC std_ss [],
-           ALL_TAC]
-    THEN PROVE_TAC [Lrules,trules,lrules,Lemma2]);
+val Theorem2 = Q.store_thm ("Theorem2",
+`!P A. MTRACE P A ==> ?Q. TRANSIT P A Q /\ TERMINAL Q`,
+ PURE_ONCE_REWRITE_TAC [TERMINAL_DEF] 
+   THEN MTRACE_INDUCT_TAC THEN REPEAT GEN_TAC THENL
+   [EXISTS_SEARCH_TAC (--`Nil`--),
+    MAP_EVERY EXISTS_SEARCH_TAC [(--`Q:agent`--),(--`P:agent`--)],
+    TRANSIT_CASES_TAC (--`TRANSIT P A Q'`--) THENL
+      [EXISTS_SEARCH_TAC (--`Sum P Q`--),
+       MAP_EVERY EXISTS_SEARCH_TAC [(--`Q':agent`--), (--`Q'':agent`--)]],
+    TRANSIT_CASES_TAC (--`TRANSIT Q A Q'`--) THENL
+      [EXISTS_SEARCH_TAC (--`Sum P Q`--),
+       MAP_EVERY EXISTS_SEARCH_TAC [(--`Q':agent`--), (--`Q'':agent`--)]], 
+    IMP_RES_TAC Lemma2 THEN EXISTS_SEARCH_TAC (--`Prod Q' Q''`--)]);
 
 (* ===================================================================== *)
 (* Theorem3: The transition and maximal trace semantics "agree".	 *)
@@ -286,8 +436,10 @@ val Theorem2 = store_thm ("Theorem2",
 val Theorem3 =
     store_thm
     ("Theorem3",
-     --`!P A. MTRACE P A = ?Q. TRANSIT P A Q /\ TERMINAL Q`--,
-    PROVE_TAC [Theorem2,Theorem1]);
+     (--`!P A. MTRACE P A = ?Q. TRANSIT P A Q /\ TERMINAL Q`--),
+     REPEAT (EQ_TAC ORELSE STRIP_TAC) THENL
+     [MATCH_MP_TAC Theorem2 THEN FIRST_ASSUM ACCEPT_TAC,
+      IMP_RES_TAC Theorem1]);
 
 
 (* ===================================================================== *)
@@ -300,9 +452,9 @@ val Theorem3 =
 (* --------------------------------------------------------------------- *)
 
 val MEQUIV_DEF =
-    new_infixl_definition
-    ("MEQUIV_DEF",
-     (--`MEQUIV P Q = (!A. MTRACE P A = MTRACE Q A)`--),725);
+ new_infixl_definition 
+    ("MEQUIV_DEF",    
+     (--`MEQUIV P Q = !A. MTRACE P A = MTRACE Q A`--),701);
 
 (* --------------------------------------------------------------------- *)
 (* Bisimulation equivalence.  A binary relation s:agent->agent->bool is  *)
@@ -313,16 +465,15 @@ val MEQUIV_DEF =
 (* --------------------------------------------------------------------- *)
 
 val SIM_DEF =
-    new_definition
-    ("SIM_DEF",
-     (--`SIM s =
-      !P Q. s P Q ==>
-            !a P'. TRANS P a P' ==> ?Q'. TRANS Q a Q' /\ s P' Q'`--));
+ Q.new_definition 
+  ("SIM_DEF",
+   `SIM s = 
+      !P Q. s P Q ==> !a P'. TRANS P a P' ==> ?Q'. TRANS Q a Q' /\ s P' Q'`);
 
 val BEQUIV_DEF =
-    new_infixl_definition
+    new_infixl_definition 
     ("BEQUIV_DEF",
-     (--`BEQUIV P Q = ?s. SIM s /\ s P Q /\ SIM(\x y. s y x)`--),725);
+     (--`BEQUIV P Q = ?s. SIM s /\ s P Q /\ SIM(\x y. s y x)`--),701);
 
 
 (* --------------------------------------------------------------------- *)
@@ -332,3 +483,5 @@ val BEQUIV_DEF =
 val _ = export_theory();
 
 end;
+
+
